Add support for sized (Word) integers, and invariants for IntVal.

Values.thy
@@ -7,10 +7,51 @@ begin
 
 type_synonym objref = "nat option"
 
+(* Java supports 64, 32, 16, 8 signed ints, plus 1 bit (boolean) ints.
+   Our Value type models this by keeping the value as an infinite precision signed int,
+   but also carrying along the number of bits allowed.
+   So each (IntVal b v) should satisfy the invariants:
+      b in {1,8,16,32,64} and
+      (b > 1 \<Longrightarrow> v == signed (signed_take_bit b v))
+*)
+type_synonym int64 = "64 word"   (* long *)
+type_synonym int32 = "32 word"   (* int *)
+type_synonym int16 = "16 word"   (* short *)
+type_synonym int8 = "8 word"   (* char *)
+type_synonym int1 = "1 word"   (* boolean *)
+
 datatype Value  =
   UndefVal |
-  IntVal (v_bits: int) (v_int: int) |
-  FloatVal (v_bits: int) (v_float: float) |
+  IntVal (v_bits: nat) (v_int: int) |
+  FloatVal (v_bits: nat) (v_float: float) |
   ObjRef objref
 
+
+fun no_overflow_n :: "nat \<Rightarrow> int \<Rightarrow> bool" where
+  "no_overflow_n b val = ((-(2^(b-1)) \<le> val) \<and> (val < (2^(b-1))))"
+
+fun wff_value :: "Value \<Rightarrow> bool" where
+  "wff_value (IntVal b v) = 
+    (b \<in> {1,8,16,32,64} \<and>
+    (b = 1 \<longrightarrow> (v = 0 \<or> v = 1)) \<and>
+    (b > 1 \<longrightarrow> no_overflow_n b v))" |
+  "wff_value _ = True"
+
+(* boolean values *)
+lemma "\<not> (wff_value (IntVal 1 (-1)))" by simp
+lemma wff_false: "wff_value (IntVal 1 0)" by simp
+lemma wff_true: "wff_value (IntVal 1 1)" by simp
+lemma "\<not> (wff_value (IntVal 1 2))" by simp
+
+value "(-7::int) div (4::int)"   (* gives -2.  Truncates towards negative infinity, unlike Java. *)
+value "(-7::int) mod (4::int)"   (* gives 1.  Whereas Java gives -3. *)
+
+(* byte values *)
+lemma wff_byte__neg129: "i < -128 \<longrightarrow> \<not> (wff_value (IntVal 8 i))" by simp
+lemma wff_byte__neg: "-128 \<le> i \<and> i < 0 \<longrightarrow> wff_value (IntVal 8 i)" by simp
+lemma wff_byte_0: "wff_value (IntVal 8 0)" by simp
+lemma wff_byte_127: "0 < i \<and> i < 128 \<longrightarrow> wff_value (IntVal 8 i)" by simp
+lemma wff_byte_128: "i \<ge> 128 \<longrightarrow> \<not> (wff_value (IntVal 8 i))" by simp
+
+value "sint(word_of_int (1) :: int1)"
 end
